utp/utp_hoare.thy
@@ -1,7 +1,9 @@
 subsection {* Relational Hoare calculus *}
 
 theory utp_hoare
-imports utp_rel_laws
+  imports 
+    utp_rel_laws
+    utp_theory
 begin
 
 named_theorems hoare and hoare_safe
@@ -89,7 +91,8 @@ lemma approx_chain:
   "(\<Sqinter>n::nat. \<lceil>p \<and> v <\<^sub>u \<guillemotleft>n\<guillemotright>\<rceil>\<^sub><) = \<lceil>p\<rceil>\<^sub><"
   by (rel_auto)
 
-text {* Total correctness law for Hoare logic *}
+text {* Total correctness law for Hoare logic, based on constructive chains. This is limited to
+  variants that have naturals numbers as their range. *}
     
 lemma while_term_hoare_r:
   assumes "\<And> z::nat. \<lbrace>p \<and> b \<and> v =\<^sub>u \<guillemotleft>z\<guillemotright>\<rbrace>S\<lbrace>p \<and> v <\<^sub>u \<guillemotleft>z\<guillemotright>\<rbrace>\<^sub>u"
@@ -143,5 +146,21 @@ lemma while_vrt_hoare_r [hoare_safe]:
   apply (simp add: while_vrt_def)
   apply (rule while_term_hoare_r[where v="v", OF assms(1)]) 
 done
+  
+text {* General total correctness law based on well-founded induction *}
+  
+lemma uwhile_total_rule:
+  assumes WF: "wf R"
+  assumes I0: "`Pre \<Rightarrow> I`"
+  assumes induct_step:"\<And> st. (\<lceil>b \<and> p \<and> e =\<^sub>u \<guillemotleft>st\<guillemotright> \<rceil>\<^sub>< \<Rightarrow> (\<lceil>p \<and> (e, \<guillemotleft>st\<guillemotright>)\<^sub>u \<in>\<^sub>u \<guillemotleft>R\<guillemotright> \<rceil>\<^sub>>)) \<sqsubseteq> Q"  
+  assumes PHI:"`\<not> \<lceil>b\<rceil>\<^sub>< \<and> \<lceil>p\<rceil>\<^sub>< \<Rightarrow> \<lceil>Post\<rceil>\<^sub>>`"  
+  shows "\<lbrace>Pre\<rbrace>while\<^sub>\<bottom> b invr p do Q od\<lbrace>Post\<rbrace>\<^sub>u"
+unfolding hoare_r_def while_inv_bot_def while_bot_def
+proof (rule rec_total_utp_rule[where e=e, OF WF])
+  show "Monotonic (\<lambda>X. Q ;; X \<triangleleft> b \<triangleright>\<^sub>r II)"
+    by (simp add: closure)
+  show "\<And>st. (\<lceil>Pre\<rceil>\<^sub>< \<and> \<lceil>e\<rceil>\<^sub>< =\<^sub>u \<guillemotleft>st\<guillemotright> \<Rightarrow> \<lceil>Post\<rceil>\<^sub>>) \<sqsubseteq> Q ;; (\<lceil>Pre\<rceil>\<^sub>< \<and> (\<lceil>e\<rceil>\<^sub><, \<guillemotleft>st\<guillemotright>)\<^sub>u \<in>\<^sub>u \<guillemotleft>R\<guillemotright> \<Rightarrow> \<lceil>Post\<rceil>\<^sub>>) \<triangleleft> b \<triangleright>\<^sub>r II"
+    apply (rule cond_refine_rel)
+oops
   
 end
